theories/sim/right_step.v
@@ -8,7 +8,7 @@ Set Default Proof Using "Type".
 Lemma sim_body_copy_right_1
   fs ft (r: resUR) k (h: heapletR) n l t s es σs σt Φ
   (* we know we're going to read s *)
-  (UNIQUE: r.1 !! t ≡ Some (k, h))
+  (UNIQUE: r.(rtm) !! t ≡ Some (k, h))
   (InD: h !! l ≡ Some (to_agree s))
   (IN: tag_in_stack σt l t) :
   (σt.(shp) !! l = Some s → r ⊨{n,fs,ft} (es, σs) ≥ (#[s%S], σt) : Φ : Prop) →
